chore: progress

SSA/Projects/CIRCT/Handshake-to-DC/ForkToken.lean
@@ -22,7 +22,7 @@ namespace Stream.Bisim
 unseal String.splitOnAux in
 def forkToken := [DCxComb_com| {
   ^entry(%0: !TokenStream):
-    %dcFork = "DCxCombOp.fork" (%0) : (!TokenStream) -> (!TokenStream2)
+    %dcFork = "DCxComb.fork" (%0) : (!TokenStream) -> (!TokenStream2)
     "return" (%dcFork) : (!TokenStream2) -> ()
   }]
 
@@ -35,11 +35,11 @@ def forkToken := [DCxComb_com| {
 def ofList (vals : List (Option α)) : Stream α :=
   fun i => (vals.get? i).join
 
-def x : DCOp.TokenStream := ofList [some (), none, some (), some (), none]
+def x : DCxCombOp.TokenStream := ofList [some (), none, some (), some (), none]
 
-def test : DCOp.TokenStream × DCOp.TokenStream :=
+def test : DCxCombOp.TokenStream × DCxCombOp.TokenStream :=
   forkToken.denote (Ctxt.Valuation.ofHVector (.cons x <| .nil))
 
 open Ctxt in
-theorem equiv_forkToken (streamT : DCOp.TokenStream) :
-  (Handshake.fork streamT).fst ~ (forkToken.denote (Valuation.ofHVector (.cons streamT <| .nil))).fst := by sorry
+theorem equiv_forkToken (streamT : DCxCombOp.TokenStream) :
+  (HandshakeOp.fork streamT).fst ~ (forkToken.denote (Valuation.ofHVector (.cons streamT <| .nil))).fst := by sorry
