SSA/Projects/CIRCT/DCxComb/Semantics.lean
@@ -26,6 +26,8 @@ def popReady (s : ValueStream (BitVec w)) (n : Nat) : BitVec w :=
   else
     0#w
 
+def pushReady (v : BitVec w) (n : Nat): (ValueStream (BitVec n)) := CIRCTStream.Stream.ofList [(v.setWidth n)]
+
 def unpack (x : ValueStream (BitVec w)) : ValueStream (BitVec w) × TokenStream :=
   Stream.corec₂ (β := Stream (BitVec w)) (x)
     fun x => Id.run <| do
@@ -57,13 +59,22 @@ def fork (x : TokenStream) : TokenStream × TokenStream  :=
     fun x => Id.run <| do
       (x 0, x 0, x.tail)
 
-def join (x y : TokenStream) : TokenStream  :=
+def add {w : Nat} (l : List (BitVec w)) : BitVec w :=
+  List.foldr BitVec.add (0#w) l
+
+def joinTwo (x y : TokenStream) : TokenStream  :=
   Stream.corec (β := TokenStream × TokenStream) (x, y) fun ⟨x, y⟩ =>
     match x 0, y 0 with
     | some _, some _ => (some (), (x.tail, y.tail))
     | some _, none => (none, (x, y.tail))
     | none, some _ => (none, (x.tail, y))
     | none, none => (none, (x.tail, y.tail))
+
+def join (l : List TokenStream) : TokenStream :=
+  if hz : 0 < l.length then
+    l.foldl joinTwo l[0]
+  else
+    Stream.ofList []
 
 def merge (x y : TokenStream) : ValueStream (BitVec 1) :=
   Stream.corec (β := TokenStream × TokenStream) (x, y) fun ⟨x, y⟩ =>
@@ -126,10 +137,6 @@ instance : ToString IcmpPredicate where
   | .ugt => "ugt"
   | .uge => "uge"
 
-/-- Variadic `add` operation with a list of bitvectors with width `w` as input -/
-def add {w : Nat} (l : List (BitVec w)) : BitVec w :=
-  List.foldr BitVec.add (0#w) l
-
 /-- Variadic `and` operation with a list of bitvectors with width `w` as input -/
 def and {w : Nat} (l : List (BitVec w)) : BitVec w :=
   List.foldr BitVec.and (0#w) l
@@ -148,34 +155,34 @@ def extract (x : BitVec w) (lb : Nat) : BitVec (w - lb) :=
   BitVec.truncate (w - lb) (BitVec.ushiftRight x lb)
 
 /-- Boolean comparison between two input BitVecs -/
-def icmp {w : Nat} (p : IcmpPredicate) (x y : BitVec w) : Bool :=
+def icmp {w : Nat} (p : IcmpPredicate) (x y : BitVec w) : BitVec 1 :=
   match p with
-  | .eq  => (x == y)
-  | .ne => (x != y)
-  | .sgt => (y.slt x)
-  | .sge => (y.sle x)
-  | .slt => (x.slt y)
-  | .sle => (x.sle y)
-  | .ugt => (x > y)
-  | .uge => (x ≥ y)
-  | .ult => (x < y)
-  | .ule => (x ≤ y)
+  | .eq  => BitVec.ofBool (x == y)
+  | .ne => BitVec.ofBool (x != y)
+  | .sgt => BitVec.ofBool (y.slt x)
+  | .sge => BitVec.ofBool (y.sle x)
+  | .slt => BitVec.ofBool (x.slt y)
+  | .sle => BitVec.ofBool (x.sle y)
+  | .ugt => BitVec.ofBool (x > y)
+  | .uge => BitVec.ofBool (x ≥ y)
+  | .ult => BitVec.ofBool (x < y)
+  | .ule => BitVec.ofBool (x ≤ y)
 
 /-- Variadic `mul` operation with a list of bitvectors with width `w` as input -/
 def mul {w : Nat} (l : List (BitVec w)) : BitVec w :=
   List.foldr BitVec.mul (1#w) l
 
 /- Generic `mux` operation for any types α, β -/
-def mux (x : BitVec w₁) (y : BitVec w₂) (cond : Bool) : BitVec w₁ ⊕ BitVec w₂ :=
-  if cond then .inl x else .inr y
+def mux (x : BitVec w₁) (y : BitVec w₂) (cond : BitVec 1) : BitVec w₁ ⊕ BitVec w₂ :=
+  if cond.msb then .inl x else .inr y
 
 /-- Variadic `or` operation with a list of bitvectors with width `w` as input -/
 def or {w : Nat} (l : List (BitVec w)) : BitVec w :=
   List.foldr BitVec.or (BitVec.zero w) l
 
 /-- Returns boolean parity value of BitVec `x` -/
-def parity (x : BitVec w) : Bool :=
-  (BitVec.umod x 2#w) == 1
+def parity (x : BitVec w) : BitVec 1 :=
+  BitVec.ofBool ((BitVec.umod x 2#w) == 1)
 
 /-- Replicate input BitVec `x` `n` times -/
 def replicate (x : BitVec w) (n : Nat) : BitVec (w * n) :=
